src/app/contracts/full-example.fst
@@ -7,18 +7,23 @@ open Zen.Cost
 module ET = Zen.ErrorT
 
 val cf: txSkeleton -> string -> cost nat 1
-let cf _ _ = ret 277
+let cf _ _ = ret 149
 
-val main: txSkeleton -> hash -> string -> cost (result txSkeleton) 277
+val main: txSkeleton -> hash -> string -> cost (result txSkeleton) 149
 let main txSkeleton contractHash command =
-let zenToken:asset = hashFromBase64 "AAAAAAAAAAAAAAAAAAAAAAAAAAAAAAAAAAAAAAAAAAA=" in
-let pk = hashFromBase64 "DYggLLPq6eXj1YxjiPQ5dSvb/YVqAVNf8Mjnpc9P9BI=" in
+let spend = {
+  asset=hashFromBase64 "AAAAAAAAAAAAAAAAAAAAAAAAAAAAAAAAAAAAAAAAAAA=";
+  amount=1000UL
+  } in
+  let lock = ContractLock contractHash in
 
-let! tokens = getAvailableTokens zenToken txSkeleton in
+  let output = { lock=lock; spend=spend } in
 
-let txSkeleton =
-    lockToContract ({asset=zenToken;amount=tokens}) contractHash txSkeleton
-    >>= mint tokens contractHash
-    >>= lockToPubKey ({asset=contractHash;amount=tokens}) pk in
+  let pInput = {
+    txHash = hashFromBase64 "AAAAAAAAAAAAAAAAAAAAAAAAAAAAAAAAAAAAAAAAAAA=";
+    index = 0ul
+    }, output in
 
-ET.retT txSkeleton
+    let txSkeleton1 = addInput pInput txSkeleton in
+    let txSkeleton2 = txSkeleton1 >>= lockToContract spend.asset spend.amount contractHash in
+    ET.retT txSkeleton2
