src/app/contracts/dorons-contract.fst
@@ -1,0 +1,24 @@
+open Zen.Types
+open Zen.Vector
+open Zen.Util
+open Zen.Base
+open Zen.Cost
+
+module ET = Zen.ErrorT
+
+val cf: txSkeleton -> string -> cost nat 1
+let cf _ _ = ret 277
+
+val main: txSkeleton -> hash -> string -> cost (result txSkeleton) 277
+let main txSkeleton contractHash command =
+let zenToken:asset = hashFromBase64 "AAAAAAAAAAAAAAAAAAAAAAAAAAAAAAAAAAAAAAAAAAA=" in
+let pk = hashFromBase64 "DYggLLPq6eXj1YxjiPQ5dSvb/YVqAVNf8Mjnpc9P9BI=" in
+
+let! tokens = getAvailableTokens zenToken txSkeleton in
+
+let txSkeleton =
+    lockToContract ({asset=zenToken;amount=tokens}) contractHash txSkeleton
+    >>= mint tokens contractHash
+    >>= lockToPubKey ({asset=contractHash;amount=tokens}) pk in
+
+ET.retT txSkeleton
